\documentclass[12pt,letterpaper]{article}
\usepackage{fullpage}
\usepackage[top=2cm, bottom=4.5cm, left=2.5cm, right=2.5cm]{geometry}
\usepackage{amsmath,amsthm,amsfonts,amssymb,amscd}

\title{Logistic Regression}
\author{Chi Nguyen}
\date{August 2022}

\begin{document}
\maketitle
\section{Proof: \(\frac{\delta L}{\delta W} = \frac{1}{N}X^T(\hat{y}-y)\)}
    \[L = -\frac{1}{N}[y\log\hat{y}+(1-y)\log(1-\hat{y})]\]
    
    \begin{equation*}
        \rightarrow
        \frac{\delta L}{\delta \hat{y}} = -\frac{1}{N}(\frac{y}{\hat{y}}-\frac{1-y}{1-\hat{y}})
                                          = \frac{1}{N}\frac{\hat{y}-y}{\hat{y}(1-\hat{y})}
    \end{equation*}

    $$X = \begin{bmatrix}
        1 & x{_1}^{(1)} & x{_2}^{(1)}\\
        1 & x{_1}^{(2)} & x{_2}^{(2)}\\
        ... & ... & ...\\
        1 & x{_1}^{(n)} & x{_2}^{(n)}\\
        \end{bmatrix},
    y = \begin{bmatrix}
            y_1\\
            y_2\\
            ...\\
            y_n
          \end{bmatrix},
    W = \begin{bmatrix}
            w_0\\
            w_1\\
            w_2
          \end{bmatrix}$$
    
    $$\hat{y} = \sigma(XW) = \frac{1}{1 + e^{-XW}}$$
    \begin{equation*}
        \begin{split}
        \frac{\delta \hat{y}}{\delta w} &= X^{T} \frac{e^{-XW}}{(1 + e^{-XW})^2}\\
                                        &= X^{T} \frac{1}{1 + e^{-XW}} (1 - \frac{1}{1 + e^{-XW}})\\
                                        &= X^{T} \hat{y}(1 - \hat{y})
        \end{split}
    \end{equation*}
    

    \begin{equation*}
        \frac{\delta L}{\delta W} = \frac{\delta L}{\delta \hat{y}} \frac{\delta \hat{y}}{\delta w}
                                  = \frac{1}{N} X^T (\hat{y}-y)
    \end{equation*}


\pagebreak                  
\section{Proof: MSE Loss is non-convex, BCE Loss is convex with LR}
    MSE: $L = (\hat{y} - y)^2$
    \begin{align*}
        \frac{\delta L}{\delta \hat{y}} &= 2(\hat{y}-y)\\
        \frac{\delta \hat{y}}{\delta W} &= -X^{T} \hat{y}(1 - \hat{y})\\
        \rightarrow
        \frac{\delta L}{\delta W} &= -2X^T(\hat{y}-y)\hat{y}(1 - \hat{y})\\
                                  &= -2X^T(\hat{y}^2-y\hat{y}-\hat{y}^3+y\hat{y}^2)\\
        \rightarrow
        \frac{\delta^2L}{\delta^2W} &= 2(X^T)^2\hat{y}(1-\hat{y})(2\hat{y}-y-3\hat{y}^2+y\hat{y})
    \end{align*}
    
    \(\hat{y} \in (0, 1) \rightarrow \hat{t}(1-\hat{y})>0 \rightarrow 2(X^T)^2\hat{y}(1-\hat{y})>0\)\\
    When y=0: 
    \begin{equation*}
        2\hat{y}-y-3\hat{y}^2+y\hat{y} = 2\hat{y} - 3\hat{y}^2 \ngeq 0 \; \forall \hat{y}
    \end{equation*}
    When y=1: 
    \begin{equation*}
        2\hat{y}-y-3\hat{y}^2+y\hat{y} = -3\hat{y}^2 +3\hat{y} -1 < 0 \; \forall \hat{y}
    \end{equation*}
    \Rightarrow \(\frac{\delta^2L}{\delta^2W} \ngeq 0\) \forall \hat{y} \Rightarrow \text{non convex}\\

    BCE: \(L = -[ylog\hat{y} + (1-y)log(1- \hat{y})]\)
    \begin{align*}
        \frac{\delta L}{\delta W} &=  X^T (\hat{y}-y)\\
        \rightarrow
        \frac{\delta^2L}{\delta^2W} &= (X^T)^2\hat{y}(1-\hat{y}) > 0 \; \forall \hat{y} \Rightarrow convex
    \end{align*}
    
\end{document}
